NCML/CK/Frame/BBox.lean
@@ -1,0 +1,73 @@
+module
+
+public import NCML.CK.Frame.SymmetricMRel
+public import NCML.CK.Frame.ForwardConfluent
+
+@[expose] public section
+
+namespace CK
+
+variable {κ : Type*}
+variable {A : BDFormula}
+
+namespace Frame
+
+variable {F : Frame κ}
+
+class BBox (F : Frame κ) : Prop where
+  bBox : ∀ {x y z : F.World}, x ⊏ y → y ≼ z → ∃ w, z ⊏ w ∧ (F.Infallible w → x ≼ w)
+
+lemma BBox.bBox' [F.BBox] : ∀ {x y z : F.World}, x ⊏ y → y ≼ z →
+  ∃ w, z ⊏ w ∧ (x ≼ w ∨ F.Fallible w) := by
+  intro x y z Mxy Iyz;
+  obtain ⟨w, Mzw, hw⟩ := bBox Mxy Iyz;
+  refine ⟨w, Mzw, ?_⟩;
+  by_cases hFallible : F.Fallible w;
+  . right;
+    exact hFallible;
+  . left;
+    exact hw hFallible;
+
+export BBox (bBox bBox')
+
+instance [F.SymmetricMRel] [F.ForwardConfluent] : F.BBox where
+  bBox Mxy Iyz := by
+    obtain ⟨w, Ixw, Mzw⟩ := forward_confluent (symm_mRel Mxy) Iyz;
+    exact ⟨w, Mzw, fun _ => Ixw⟩;
+
+lemma frameValidate_BBox_of_frame_BBox [F.BBox] : F ⊧ (A 🡒 □◇A) := by
+  intro V V_per V_fal x y Ixy hyA z w Iyz Mzw v Iwv;
+  obtain ⟨u, Mvu, Izu | hu⟩ := bBox' Mzw Iwv;
+  . exact ⟨u, Mvu, forces_persistent hyA (Trans.trans Iyz Izu)⟩;
+  . exact ⟨u, Mvu, forces_of_fallible hu⟩;
+
+lemma frame_BBox_of_frameValidate_BBox (h : F ⊧ (#0 🡒 □◇(#0))) : F.BBox where
+  bBox {x y z} Mxy Iyz := by
+    let M : Model κ := {
+      toFrame := F,
+      val := fun w _ => F.Infallible w → x ≼ w,
+      val_persistent := by
+        rintro w v a h Iwv Iv;
+        trans w;
+        . exact h $ infallible_iRel Iv Iwv;
+        . assumption;
+      fallible_val := by grind;
+    }
+    have hxA : x ⊩[M] (#0) := fun _ => refl x;
+    exact h M.val M.val_persistent M.fallible_val x x (refl x) hxA x y (refl x) Mxy z Iyz;
+
+theorem frame_BBox_TFAE : List.TFAE [
+  F.BBox,
+  ∀ A : BDFormula, F ⊧ (A 🡒 □◇A),
+  F ⊧ (#0 🡒 □◇(#0)),
+] := by
+  tfae_have 1 → 2 := by intro h A; exact frameValidate_BBox_of_frame_BBox;
+  tfae_have 2 → 3 := fun h => h _
+  tfae_have 3 → 1 := frame_BBox_of_frameValidate_BBox
+  tfae_finish
+
+end Frame
+
+end CK
+
+end
