NCML/CK/Frame/BackwardConfluent.lean
@@ -1,0 +1,59 @@
+module
+
+public import NCML.CK.Frame.SymmetricMRel
+public import NCML.CK.Frame.ForwardConfluent
+
+@[expose] public section
+
+namespace CK
+
+variable {κ : Type*}
+variable {A B : BDFormula}
+
+namespace Frame
+
+variable {F : Frame κ}
+
+/-- - [Pac24, Definition 5] -/
+class BackwardConfluent (F : Frame κ) : Prop where
+  backward_confluent : ∀ {x y z : F.World}, x ⊏ y → y ≼ z → ∃ w, x ≼ w ∧ w ⊏ z
+
+export BackwardConfluent (backward_confluent)
+
+/-- - [Pac24, Proposition 10] -/
+lemma frame_ForwardConfluent_iff_frame_BackwardConfluent_of_frame_SymmetricMRel
+  [F.SymmetricMRel] :
+  F.ForwardConfluent ↔ F.BackwardConfluent := by
+  constructor;
+  · intro h;
+    constructor;
+    intro x y z Mxy Iyz;
+    obtain ⟨w, Ixw, Mzw⟩ := h.forward_confluent (symm_mRel Mxy) Iyz;
+    exact ⟨w, Ixw, symm_mRel Mzw⟩;
+  · intro h;
+    constructor;
+    intro x y z Mxy Ixz;
+    obtain ⟨w, Iyw, Mwz⟩ := h.backward_confluent (symm_mRel Mxy) Ixz;
+    exact ⟨w, Iyw, symm_mRel Mwz⟩;
+
+/--
+- [dGSC25]
+- [Pac24, Theorem 11]
+- [Pac24, Corollary 12]
+-/
+lemma frameValidate_FS_of_frame_ForwardConfluent_of_frame_BackwardConfluent
+  [F.ForwardConfluent] [F.BackwardConfluent] :
+  F ⊧ ((◇A 🡒 □B) 🡒 □(A 🡒 B)) := by
+  intro V V_per V_fal x y Ixy hy z w Iyz Mzw v Iwv hvA;
+  obtain ⟨u, Izu, Muv⟩ := backward_confluent Mzw Iwv;
+  have huDiaA : u ⊩[_] ◇A := by
+    intro x₁ Iux₁;
+    obtain ⟨y₁, Ivy₁, Mx₁y₁⟩ := forward_confluent Muv Iux₁;
+    exact ⟨y₁, Mx₁y₁, forces_persistent hvA Ivy₁⟩;
+  exact hy u (Trans.trans Iyz Izu) huDiaA u v (refl u) Muv;
+
+end Frame
+
+end CK
+
+end
