NCML/CK/Frame/FiveBox.lean
@@ -1,0 +1,93 @@
+module
+
+public import NCML.CK.Frame.EuclideanMRel
+public import NCML.CK.Frame.ForwardConfluent
+
+@[expose] public section
+
+namespace CK
+
+variable {κ : Type*}
+variable {A : BDFormula}
+
+namespace Frame
+
+variable {F : Frame κ}
+
+class FiveBox (F : Frame κ) : Prop where
+  fiveBox : ∀ {x y z : F.World}, x ⊏ y → y ≼ z →
+    ∃ w, x ≼ w ∧ ∀ v, w ⊏ v → ∃ u, z ⊏ u ∧ (F.Infallible u → v ≼ u)
+
+lemma FiveBox.fiveBox' [F.FiveBox] : ∀ {x y z : F.World}, x ⊏ y → y ≼ z →
+  ∃ w, x ≼ w ∧ ∀ v, w ⊏ v → ∃ u, z ⊏ u ∧ (v ≼ u ∨ F.Fallible u) := by
+  intro x y z Mxy Iyz;
+  obtain ⟨w, Ixw, hw⟩ := fiveBox Mxy Iyz;
+  refine ⟨w, Ixw, ?_⟩;
+  intro v Mwv;
+  obtain ⟨u, Mzu, hu⟩ := hw v Mwv;
+  refine ⟨u, Mzu, ?_⟩;
+  by_cases hFallible : F.Fallible u;
+  . right;
+    exact hFallible;
+  . left;
+    exact hu hFallible;
+
+export FiveBox (fiveBox fiveBox')
+
+instance [F.EuclideanMRel] [F.ForwardConfluent] : F.FiveBox where
+  fiveBox {x y z} Mxy Iyz := by
+    use x;
+    constructor;
+    . apply refl;
+    . intro v Mxv;
+      obtain ⟨u, Ivu, Mzu⟩ := forward_confluent (eucl_mRel Mxy Mxv) Iyz;
+      exact ⟨u, Mzu, fun _ => Ivu⟩;
+
+lemma frameValidate_FiveBox_of_frame_FiveBox [F.FiveBox] : F ⊧ (◇A 🡒 □◇A) := by
+  intro V V_per V_fal x y Ixy hy z w Iyz Mzw v Iwv;
+  obtain ⟨u, Izu, hu⟩ := fiveBox' Mzw Iwv;
+  obtain ⟨v₁, Muv₁, hv₁⟩ := hy u (Trans.trans Iyz Izu);
+  obtain ⟨u₁, Mvu₁, hu₁⟩ := hu v₁ Muv₁;
+  rcases hu₁ with Iv₁u₁ | hFallible;
+  . exact ⟨u₁, Mvu₁, forces_persistent hv₁ Iv₁u₁⟩;
+  . exact ⟨u₁, Mvu₁, forces_of_fallible hFallible⟩;
+
+lemma frame_FiveBox_of_frameValidate_FiveBox (h : F ⊧ (◇(#0) 🡒 □◇(#0))) : F.FiveBox where
+  fiveBox {x y z} Mxy Iyz := by
+    by_contra! hc;
+    obtain ⟨v, Mxv, hv⟩ := hc x (refl x);
+    have hNotFallible : ∀ u, z ⊏ u → F.Infallible u := fun u Mzu => (hv u Mzu).1;
+    let M : Model κ := {
+      toFrame := F,
+      val := fun v _ => F.Infallible v → ∀ u, v ≼ u → ¬(z ⊏ u),
+      val_persistent := by
+        rintro v v₁ a hv Ivv₁ Iv₁ u Iv₁u;
+        exact hv (infallible_iRel Iv₁ Ivv₁) u (Trans.trans Ivv₁ Iv₁u);
+      fallible_val := by grind;
+    }
+    have hxDia : x ⊩[M] ◇(#0) := by
+      intro w Ixw;
+      obtain ⟨v, Mxv, hv⟩ := hc w Ixw;
+      refine ⟨v, Mxv, ?_⟩;
+      intro _ u Ivu Mzu;
+      exact (hv u Mzu).2 Ivu;
+    have hxBoxDia : x ⊩[M] □◇(#0) :=
+      h M.val M.val_persistent M.fallible_val x x (refl x) hxDia;
+    obtain ⟨u, Mzu, hu⟩ := hxBoxDia x y (refl x) Mxy z Iyz;
+    exact hu (hNotFallible u Mzu) u (refl u) Mzu;
+
+theorem frame_FiveBox_TFAE : List.TFAE [
+  F.FiveBox,
+  ∀ A : BDFormula, F ⊧ (◇A 🡒 □◇A),
+  F ⊧ (◇(#0) 🡒 □◇(#0)),
+] := by
+  tfae_have 1 → 2 := by intro h A; exact frameValidate_FiveBox_of_frame_FiveBox;
+  tfae_have 2 → 3 := fun h => h _
+  tfae_have 3 → 1 := frame_FiveBox_of_frameValidate_FiveBox
+  tfae_finish
+
+end Frame
+
+end CK
+
+end
