NCML/CK/Frame/FiveDia.lean
@@ -1,0 +1,77 @@
+module
+
+public import NCML.CK.Frame.EuclideanMRel
+
+@[expose] public section
+
+namespace CK
+
+variable {κ : Type*}
+variable {A : BDFormula}
+
+namespace Frame
+
+variable {F : Frame κ}
+
+class FiveDia (F : Frame κ) : Prop where
+  fiveDia : ∀ {x y : F.World}, x ⊏ y → F.Infallible y →
+    ∃ z, x ≼ z ∧ ∀ w, z ⊏ w → ∃ v u, w ≼ v ∧ v ⊏ u ∧ u ≼ y
+export FiveDia (fiveDia)
+
+instance [F.EuclideanMRel] : F.FiveDia where
+  fiveDia {x y} Mxy _ := by
+    use x;
+    constructor;
+    . apply refl;
+    . intro w Mxw;
+      use w, y;
+      and_intros;
+      . apply refl;
+      . exact eucl_mRel Mxw Mxy;
+      . apply refl;
+
+lemma frameValidate_FiveDia_of_frame_FiveDia [F.FiveDia] : F ⊧ (◇(□A) 🡒 □A) := by
+  intro V V_per V_fal x y Ixy hy z w Iyz Mzw;
+  by_cases hFallible : F.Fallible w;
+  . exact forces_of_fallible hFallible;
+  . obtain ⟨v, Izv, hv⟩ := fiveDia Mzw hFallible;
+    obtain ⟨u, Mvu, hu⟩ := hy v (Trans.trans Iyz Izv);
+    obtain ⟨v₁, u₁, Iuv₁, Mv₁u₁, Iu₁w⟩ := hv u Mvu;
+    exact forces_persistent (hu v₁ u₁ Iuv₁ Mv₁u₁) Iu₁w;
+
+lemma frame_FiveDia_of_frameValidate_FiveDia (h : F ⊧ (◇(□(#0)) 🡒 □(#0))) : F.FiveDia where
+  fiveDia {x y} Mxy hy := by
+    by_contra! hc;
+    let M : Model κ := {
+      toFrame := F,
+      val := fun z _ => F.Infallible z → ¬(z ≼ y),
+      val_persistent := by
+        rintro z z₁ a hz Izz₁ Iz₁ hz₁y;
+        exact hz (infallible_iRel Iz₁ Izz₁) (Trans.trans Izz₁ hz₁y);
+      fallible_val := by grind;
+    }
+    have hxDiaBox : x ⊩[M] ◇(□(#0)) := by
+      intro z Ixz;
+      obtain ⟨w, Mzw, hw⟩ := hc z Ixz;
+      use w, Mzw;
+      intro v u Iwv Mvu _;
+      exact hw v u Iwv Mvu;
+    have hxBox : x ⊩[M] □(#0) :=
+      h M.val M.val_persistent M.fallible_val x x (refl x) hxDiaBox;
+    exact hxBox x y (refl x) Mxy hy (refl y);
+
+theorem frame_FiveDia_TFAE : List.TFAE [
+  F.FiveDia,
+  ∀ A : BDFormula, F ⊧ (◇(□A) 🡒 □A),
+  F ⊧ (◇(□(#0)) 🡒 □(#0)),
+] := by
+  tfae_have 1 → 2 := by intro h A; exact frameValidate_FiveDia_of_frame_FiveDia;
+  tfae_have 2 → 3 := fun h => h _
+  tfae_have 3 → 1 := frame_FiveDia_of_frameValidate_FiveDia
+  tfae_finish
+
+end Frame
+
+end CK
+
+end
