NCML/CK/Frame/ForwardConfluent.lean
@@ -1,0 +1,60 @@
+module
+
+public import NCML.CK.Semantics
+
+@[expose] public section
+
+namespace CK
+
+variable {κ : Type*}
+variable {A B : BDFormula}
+
+namespace Frame
+
+variable {F : Frame κ}
+
+/-- - [Pac24, Definition 5] -/
+class ForwardConfluent (F : Frame κ) : Prop where
+  forward_confluent : ∀ {x y z : F.World}, x ⊏ y → x ≼ z → ∃ w, y ≼ w ∧ z ⊏ w
+
+export ForwardConfluent (forward_confluent)
+
+end Frame
+
+namespace Model
+
+open CK.Frame
+
+variable {M : Model κ}
+variable {x : M.World}
+
+/-- - [Pac24, Proposition 6] -/
+lemma dia_iff_forward_of_forwardConfluent [M.ForwardConfluent] : x ⊩[_] ◇A ↔ ∃ y, x ⊏ y ∧ y ⊩[_] A := by
+  constructor;
+  · intro h;
+    exact h x (refl x);
+  · rintro ⟨y, Mxy, hyA⟩ z Ixz;
+    obtain ⟨w, Iyw, Mzw⟩ := forward_confluent Mxy Ixz;
+    exact ⟨w, Mzw, forces_persistent hyA Iyw⟩;
+
+end Model
+
+namespace Frame
+
+variable {F : Frame κ}
+
+/--
+- [dGSC25]
+- [Pac24, Theorem 11]
+- [Pac24, Corollary 12]
+-/
+lemma frameValidate_DP_of_frame_ForwardConfluent [F.ForwardConfluent] :
+  F ⊧ (◇(A ⋎ B) 🡒 (◇A ⋎ ◇B)) := by
+  intro V V_per V_fal x y _ hy;
+  grind [Model.dia_iff_forward_of_forwardConfluent];
+
+end Frame
+
+end CK
+
+end
