NCML/CK/Frame/FourBox.lean
@@ -1,0 +1,73 @@
+module
+
+public import NCML.CK.Frame.TransitiveMRel
+public import NCML.CK.Frame.BackwardConfluent
+
+@[expose] public section
+
+namespace CK
+
+variable {κ : Type*}
+variable {A : BDFormula}
+
+namespace Frame
+
+variable {F : Frame κ}
+
+class FourBox (F : Frame κ) : Prop where
+  fourBox : ∀ {x y z w : F.World}, x ⊏ y → y ≼ z → z ⊏ w →
+    F.Infallible w → ∃ v u, x ≼ v ∧ v ⊏ u ∧ u ≼ w
+
+lemma FourBox.fourBox' [F.FourBox] : ∀ {x y z w : F.World}, x ⊏ y → y ≼ z → z ⊏ w →
+  F.Fallible w ∨ ∃ v u, x ≼ v ∧ v ⊏ u ∧ u ≼ w := by
+  intro x y z w Mxy Iyz Mzw;
+  by_cases hFallible : F.Fallible w;
+  . left;
+    exact hFallible;
+  . right;
+    exact fourBox Mxy Iyz Mzw hFallible;
+
+export FourBox (fourBox fourBox')
+
+instance [F.TransitiveMRel] [F.BackwardConfluent] : F.FourBox where
+  fourBox {x y z w} Mxy Iyz Mzw _ := by
+    obtain ⟨v, Ixv, Mvz⟩ := backward_confluent Mxy Iyz;
+    exact ⟨v, w, Ixv, trans_mRel Mvz Mzw, refl w⟩;
+
+lemma frameValidate_FourBox_of_frame_FourBox [F.FourBox] : F ⊧ (□A 🡒 □□A) := by
+  intro V V_per V_fal x y Ixy hy z w Iyz Mzw v u Iwv Mvu;
+  rcases fourBox' Mzw Iwv Mvu with hu | ⟨v₁, u₁, Izv₁, Mv₁u₁, Iu₁u⟩;
+  . exact forces_of_fallible hu;
+  . exact forces_persistent (hy v₁ u₁ (Trans.trans Iyz Izv₁) Mv₁u₁) Iu₁u;
+
+lemma frame_FourBox_of_frameValidate_FourBox (h : F ⊧ (□(#0) 🡒 □□(#0))) : F.FourBox where
+  fourBox {x y z w} Mxy Iyz Mzw := by
+    let M : Model κ := {
+      toFrame := F,
+      val := fun v _ => F.Infallible v → ∃ u₁ t₁, x ≼ u₁ ∧ u₁ ⊏ t₁ ∧ t₁ ≼ v,
+      val_persistent := by
+        rintro v u a h Ivu Iu;
+        obtain ⟨u₁, t₁, Ixu₁, Mu₁t₁, Itv⟩ := h (infallible_iRel Iu Ivu);
+        exact ⟨u₁, t₁, Ixu₁, Mu₁t₁, Trans.trans Itv Ivu⟩;
+      fallible_val := by grind;
+    }
+    have hxBoxA : x ⊩[M] □(#0) := fun v u₁ Ixv Mvu₁ _ => ⟨v, u₁, Ixv, Mvu₁, refl u₁⟩;
+    have hxBoxBoxA : x ⊩[M] □□(#0) :=
+      h M.val M.val_persistent M.fallible_val x x (refl x) hxBoxA;
+    exact hxBoxBoxA x y (refl x) Mxy z w Iyz Mzw;
+
+theorem frame_FourBox_TFAE : List.TFAE [
+  F.FourBox,
+  ∀ A : BDFormula, F ⊧ (□A 🡒 □□A),
+  F ⊧ (□(#0) 🡒 □□(#0)),
+] := by
+  tfae_have 1 → 2 := by intro h A; exact frameValidate_FourBox_of_frame_FourBox;
+  tfae_have 2 → 3 := fun h => h _
+  tfae_have 3 → 1 := frame_FourBox_of_frameValidate_FourBox
+  tfae_finish
+
+end Frame
+
+end CK
+
+end
