NCML/CK/Frame/FourDia.lean
@@ -1,0 +1,107 @@
+module
+
+public import NCML.CK.Frame.TransitiveMRel
+
+@[expose] public section
+
+namespace CK
+
+variable {κ : Type*}
+variable {A : BDFormula}
+
+namespace Frame
+
+variable {F : Frame κ}
+
+class FourDia (F : Frame κ) : Prop where
+  fourDia : ∀ x : F.World, ∃ y, x ≼ y ∧ ∀ z, y ⊏ z → ∃ w, z ≼ w ∧
+    ∀ v, w ⊏ v → ∃ u, x ⊏ u ∧ (F.Infallible u → v ≼ u)
+
+lemma FourDia.fourDia' [F.FourDia] : ∀ x : F.World, ∃ y, x ≼ y ∧ ∀ z, y ⊏ z → ∃ w, z ≼ w ∧
+  ∀ v, w ⊏ v → ∃ u, x ⊏ u ∧ (v ≼ u ∨ F.Fallible u) := by
+  intro x;
+  obtain ⟨y, Ixy, hy⟩ := fourDia x;
+  refine ⟨y, Ixy, ?_⟩;
+  intro z Myz;
+  obtain ⟨w, Izw, hw⟩ := hy z Myz;
+  refine ⟨w, Izw, ?_⟩;
+  intro v Mwv;
+  obtain ⟨u, Mxu, hu⟩ := hw v Mwv;
+  refine ⟨u, Mxu, ?_⟩;
+  by_cases hFallible : F.Fallible u;
+  . right;
+    exact hFallible;
+  . left;
+    exact hu hFallible;
+
+export FourDia (fourDia fourDia')
+
+instance [F.TransitiveMRel] : F.FourDia where
+  fourDia x := by
+    use x;
+    constructor;
+    . apply refl;
+    . intro z Mxz;
+      use z;
+      constructor;
+      . apply refl;
+      . intro v Mzv;
+        use v;
+        constructor;
+        . exact trans_mRel Mxz Mzv;
+        . exact fun _ => refl v;
+
+lemma frameValidate_FourDia_of_frame_FourDia [F.FourDia] : F ⊧ (◇◇A 🡒 ◇A) := by
+  intro V V_per V_fal x y Ixy hy z Iyz;
+  have hz := forces_persistent hy Iyz;
+  obtain ⟨w, Izw, hw⟩ := fourDia' z;
+  obtain ⟨v, Mwv, hv⟩ := hz w Izw;
+  obtain ⟨u, Ivu, hu⟩ := hw v Mwv;
+  obtain ⟨v₁, Muv₁, hv₁⟩ := hv u Ivu;
+  obtain ⟨u₁, Mzu₁, hu₁⟩ := hu v₁ Muv₁;
+  rcases hu₁ with Ivu₁ | hFallible;
+  . exact ⟨u₁, Mzu₁, forces_persistent hv₁ Ivu₁⟩;
+  . exact ⟨u₁, Mzu₁, forces_of_fallible hFallible⟩;
+
+lemma frame_FourDia_of_frameValidate_FourDia (h : F ⊧ (◇◇(#0) 🡒 ◇(#0))) : F.FourDia where
+  fourDia x := by
+    by_contra! hc;
+    obtain ⟨z, Mxz, hz⟩ := hc x (refl x);
+    obtain ⟨v, Mzv, hv⟩ := hz z (refl z);
+    have hNotFallible : ∀ u, x ⊏ u → F.Infallible u := fun u Mxu => (hv u Mxu).1;
+    let M : Model κ := {
+      toFrame := F,
+      val := fun v _ => F.Infallible v → ∀ u, v ≼ u → ¬(x ⊏ u),
+      val_persistent := by
+        rintro v v₁ a h Ivv₁ Iv₁ u Iv₁u;
+        exact h (infallible_iRel Iv₁ Ivv₁) u (Trans.trans Ivv₁ Iv₁u);
+      fallible_val := by grind;
+    }
+    have hxDiaDia : x ⊩[M] ◇◇(#0) := by
+      intro y Ixy;
+      obtain ⟨z, Myz, hz⟩ := hc y Ixy;
+      refine ⟨z, Myz, ?_⟩;
+      intro w Izw;
+      obtain ⟨v, Mwv, hv⟩ := hz w Izw;
+      refine ⟨v, Mwv, ?_⟩;
+      intro _ u Ivu hxu;
+      exact (hv u hxu).2 Ivu;
+    have hxDia : x ⊩[M] ◇(#0) := h M.val M.val_persistent M.fallible_val x x (refl x) hxDiaDia;
+    obtain ⟨z, Mxz, hz⟩ := hxDia x (refl x);
+    exact hz (hNotFallible z Mxz) z (refl z) Mxz;
+
+theorem frame_FourDia_TFAE : List.TFAE [
+  F.FourDia,
+  ∀ A : BDFormula, F ⊧ (◇◇A 🡒 ◇A),
+  F ⊧ (◇◇(#0) 🡒 ◇(#0)),
+] := by
+  tfae_have 1 → 2 := by intro h A; exact frameValidate_FourDia_of_frame_FourDia;
+  tfae_have 2 → 3 := fun h => h _
+  tfae_have 3 → 1 := frame_FourDia_of_frameValidate_FourDia
+  tfae_finish
+
+end Frame
+
+end CK
+
+end
