NCML/CK/Frame/PBox.lean
@@ -1,0 +1,52 @@
+module
+
+public import NCML.CK.Frame.TBox
+
+@[expose] public section
+
+namespace CK
+
+variable {κ : Type*}
+
+namespace Frame
+
+variable {F : Frame κ}
+
+class PBox (F : Frame κ) : Prop where
+  pBox : ∀ {x : F.World}, F.Infallible x → ∃ y z, x ≼ y ∧ y ⊏ z ∧ F.Infallible z
+
+export PBox (pBox)
+
+instance [F.TBox] : F.PBox where
+  pBox {x} hx := by
+    obtain ⟨y, z, Ixy, Myz, Izx⟩ := tBox x hx;
+    exact ⟨y, z, Ixy, Myz, infallible_iRel hx Izx⟩;
+
+lemma frameValidate_PBox_of_frame_PBox [F.PBox] : F ⊧ (∼□⊥ : BDFormula) := by
+  intro V V_per V_fal x y Ixy hy;
+  by_contra hInfallible;
+  obtain ⟨z, w, Iyz, Mzw, hw⟩ := pBox hInfallible;
+  exact hw (hy z w Iyz Mzw);
+
+lemma frame_PBox_of_frameValidate_PBox (h : F ⊧ (∼□⊥ : BDFormula)) : F.PBox where
+  pBox {x} hx := by
+    by_contra! hc;
+    let M : Model κ := {
+      toFrame := F,
+      val := fun _ _ => True,
+      val_persistent := by intros; trivial,
+      fallible_val := by intros; trivial,
+    }
+    exact hx (h M.val M.val_persistent M.fallible_val x x (refl x) hc);
+
+theorem frame_PBox_iff_frameValidate_PBox : F.PBox ↔ F ⊧ (∼□⊥ : BDFormula) := by
+  constructor;
+  . intro _;
+    exact frameValidate_PBox_of_frame_PBox;
+  . exact frame_PBox_of_frameValidate_PBox;
+
+end Frame
+
+end CK
+
+end
