NCML/CK/Frame/SerialMRel.lean
@@ -1,0 +1,71 @@
+module
+
+public import NCML.CK.Semantics
+
+@[expose] public section
+
+namespace CK
+
+variable {κ : Type*}
+variable {A : BDFormula}
+
+namespace Frame
+
+variable {F : Frame κ}
+
+class SerialMRel (F : Frame κ) : Prop where
+  serial_mRel : ∀ x : F.World, ∃ y, x ⊏ y
+
+export SerialMRel (serial_mRel)
+
+lemma frameValidate_D_of_frame_SerialMRel [F.SerialMRel] : F ⊧ (□A 🡒 ◇A) := by
+  intro V V_per V_fal x y Ixy hyBoxA z Iyz;
+  obtain ⟨w, Mzw⟩ := serial_mRel z;
+  exact ⟨w, Mzw, hyBoxA z w Iyz Mzw⟩;
+
+lemma frameValidate_PDia_of_frame_SerialMRel [F.SerialMRel] : F ⊧ ◇⊤ := by
+  intro V V_per V_fal x y Ixy;
+  obtain ⟨z, Myz⟩ := serial_mRel y;
+  exact ⟨z, Myz, by grind⟩;
+
+lemma frame_SerialMRel_of_frameValidate_D (h : F ⊧ (□(#0) 🡒 ◇(#0))) : F.SerialMRel where
+  serial_mRel x := by
+    let M : Model κ := {
+      toFrame := F,
+      val := fun _ _ => True,
+      val_persistent := by intros; trivial,
+      fallible_val := by intros; trivial,
+    }
+    have hxBoxA : x ⊩[M] □(#0) := by intro y z _ _; trivial;
+    obtain ⟨y, Mxy, -⟩ := h M.val M.val_persistent M.fallible_val x x (refl x) hxBoxA x (refl x);
+    exact ⟨y, Mxy⟩;
+
+lemma frame_SerialMRel_of_frameValidate_PDia (h : F ⊧ ◇⊤) : F.SerialMRel where
+  serial_mRel x := by
+    let M : Model κ := {
+      toFrame := F,
+      val := fun _ _ => True,
+      val_persistent := by intros; trivial,
+      fallible_val := by intros; trivial,
+    }
+    obtain ⟨y, Mxy, -⟩ := h M.val M.val_persistent M.fallible_val x x (refl x);
+    exact ⟨y, Mxy⟩;
+
+theorem frame_SerialMRel_TFAE : List.TFAE [
+  F.SerialMRel,
+  ∀ A : BDFormula, F ⊧ (□A 🡒 ◇A),
+  F ⊧ (□(#0) 🡒 ◇(#0)),
+  F ⊧ ◇⊤,
+] := by
+  tfae_have 1 → 2 := by intro h A; exact frameValidate_D_of_frame_SerialMRel;
+  tfae_have 2 → 3 := fun h => h _
+  tfae_have 3 → 1 := frame_SerialMRel_of_frameValidate_D
+  tfae_have 1 → 4 := by intro h; exact frameValidate_PDia_of_frame_SerialMRel;
+  tfae_have 4 → 1 := frame_SerialMRel_of_frameValidate_PDia
+  tfae_finish
+
+end Frame
+
+end CK
+
+end
