NCML/CK/Frame/TBox.lean
@@ -1,0 +1,63 @@
+module
+
+public import NCML.CK.Semantics
+
+@[expose] public section
+
+namespace CK
+
+variable {κ : Type*}
+variable {A : BDFormula}
+
+namespace Frame
+
+variable {F : Frame κ}
+
+class TBox (F : Frame κ) : Prop where
+  tBox : ∀ x : F.World, F.Infallible x → ∃ y z, x ≼ y ∧ y ⊏ z ∧ z ≼ x
+
+lemma TBox.tBox' [F.TBox] : ∀ x : F.World, F.Fallible x ∨ ∃ y z, x ≼ y ∧ y ⊏ z ∧ z ≼ x := by
+  intro x;
+  by_cases hx : F.Fallible x;
+  · left;
+    exact hx;
+  · right;
+    exact tBox x hx;
+
+export TBox (tBox tBox')
+
+lemma frameValidate_TBox_of_frame_TBox [F.TBox] : F ⊧ (□A 🡒 A) := by
+  intro V V_per V_fal x y Ixy hyBoxA;
+  rcases tBox' y with hFallible | ⟨z, w, Iyz, Mzw, Iwy⟩;
+  · exact forces_of_fallible hFallible;
+  · exact forces_persistent (hyBoxA z w Iyz Mzw) Iwy;
+
+lemma frame_TBox_of_frameValidate_TBox (h : F ⊧ (□(#0) 🡒 #0)) : F.TBox where
+  tBox x hx := by
+    let M : Model κ := {
+      toFrame := F,
+      val := fun y _ => F.Infallible y → ∃ z w, x ≼ z ∧ z ⊏ w ∧ w ≼ y,
+      val_persistent := by
+        rintro y z a h Iyz hz;
+        obtain ⟨w, v, Ixw, Mwv, Ivy⟩ := h (infallible_iRel hz Iyz);
+        exact ⟨w, v, Ixw, Mwv, Trans.trans Ivy Iyz⟩;
+      fallible_val := by grind;
+    }
+    have hxBoxA : x ⊩[M] □(#0) := fun y z Ixy Myz _ => ⟨y, z, Ixy, Myz, refl z⟩;
+    exact h M.val M.val_persistent M.fallible_val x x (refl x) hxBoxA hx;
+
+theorem frame_TBox_TFAE : List.TFAE [
+  F.TBox,
+  ∀ A : BDFormula, F ⊧ (□A 🡒 A),
+  F ⊧ (□(#0) 🡒 #0),
+] := by
+  tfae_have 1 → 2 := by intro h A; exact frameValidate_TBox_of_frame_TBox;
+  tfae_have 2 → 3 := fun h => h _
+  tfae_have 3 → 1 := frame_TBox_of_frameValidate_TBox
+  tfae_finish
+
+end Frame
+
+end CK
+
+end
