NCML/CK/Frame/TDia.lean
@@ -1,0 +1,67 @@
+module
+
+public import NCML.CK.Frame.SerialMRel
+
+@[expose] public section
+
+namespace CK
+
+variable {κ : Type*}
+variable {A : BDFormula}
+
+namespace Frame
+
+variable {F : Frame κ}
+
+class TDia (F : Frame κ) : Prop where
+  tDia : ∀ x : F.World, ∃ z, x ⊏ z ∧ (F.Infallible z → x ≼ z)
+
+lemma TDia.tDia' [F.TDia] : ∀ x : F.World, ∃ z, x ⊏ z ∧ (x ≼ z ∨ F.Fallible z) := by
+  intro x;
+  grind [tDia x];
+
+export TDia (tDia tDia')
+
+instance [F.TDia] : F.SerialMRel where
+  serial_mRel x := by
+    obtain ⟨z, Mxz, -⟩ := tDia x;
+    exact ⟨z, Mxz⟩;
+
+lemma frameValidate_TDia_of_frame_TDia [F.TDia] : F ⊧ (A 🡒 ◇A) := by
+  intro V V_per V_fal x y Ixy hyA u Iyu;
+  obtain ⟨z, Muz, hz⟩ := tDia' u;
+  have huA : u ⊩[_] A := forces_persistent hyA Iyu;
+  rcases hz with Iuz | hzFallible;
+  · exact ⟨z, Muz, forces_persistent huA Iuz⟩;
+  · exact ⟨z, Muz, forces_of_fallible hzFallible⟩;
+
+lemma frame_TDia_of_frameValidate_TDia (h : F ⊧ (#0 🡒 ◇(#0))) : F.TDia where
+  tDia x := by
+    let M : Model κ := {
+      toFrame := F,
+      val := fun y _ => F.Infallible y → x ≼ y,
+      val_persistent := by
+        rintro y z a h Iyz hz;
+        trans y;
+        . exact h $ infallible_iRel hz Iyz;
+        . assumption;
+      fallible_val := by grind;
+    }
+    have hxA : x ⊩[M] (#0) := fun _ => refl _
+    exact h M.val M.val_persistent M.fallible_val x x (refl x) hxA x (refl x);
+
+theorem frame_TDia_TFAE : List.TFAE [
+  F.TDia,
+  ∀ A : BDFormula, F ⊧ (A 🡒 ◇A),
+  F ⊧ (#0 🡒 ◇(#0)),
+] := by
+  tfae_have 1 → 2 := by intro h A; exact frameValidate_TDia_of_frame_TDia;
+  tfae_have 2 → 3 := fun h => h _
+  tfae_have 3 → 1 := frame_TDia_of_frameValidate_TDia
+  tfae_finish
+
+end Frame
+
+end CK
+
+end
