NCML/CK/Logic/CK.lean
@@ -1,0 +1,19 @@
+module
+
+public import NCML.CK.Canonical
+public import NCML.CK.Soundness
+
+@[expose] public section
+
+/-- - [MdP05, Theorem 1] -/
+theorem LogicCK.mem_iff_valid {A : BDFormula} :
+  A ∈ LogicCK ↔ ∀ {κ : Type 0}, ∀ M : CK.Model κ, M ⊧ A := by
+  constructor;
+  · intro h _ M;
+    exact CK.Model.valid_of_mem_LogicCK h;
+  · contrapose!;
+    intro h;
+    obtain ⟨P, h₁⟩ := CK.exists_not_forces_of_not_mem (L := LogicCK) h;
+    exact ⟨_, CK.canonicalModel LogicCK, fun hM => h₁ (hM P)⟩;
+
+end
