NCML/CK/Logic/CKD.lean
@@ -1,0 +1,64 @@
+module
+
+public import NCML.CK.Frame.SerialMRel
+public import NCML.CK.Canonical
+public import NCML.CK.Soundness
+
+@[expose] public section
+
+open ProvableBDHilbert
+open scoped BDFormulaSet BDFormulaList
+
+namespace CK
+
+variable {κ : Type*} {M : Model κ}
+variable {A : BDFormula}
+
+namespace Model
+
+open CK.Frame
+
+lemma valid_of_mem_LogicCKD [M.SerialMRel] (hA : A ∈ LogicCKD) : M ⊧ A :=
+  valid_of_mem_logic
+    (by rintro B ⟨C, rfl⟩; exact valid_of_toFrame_valid frameValidate_D_of_frame_SerialMRel) hA
+
+lemma valid_of_mem_LogicCKPDia [M.SerialMRel] (hA : A ∈ LogicCKPDia) : M ⊧ A :=
+  valid_of_mem_logic
+    (by rintro B rfl; exact valid_of_toFrame_valid frameValidate_PDia_of_frame_SerialMRel) hA
+
+end Model
+
+variable {L : BDLogic} [L.CK]
+
+lemma serialMRel_canonicalModel (hD : ∀ {A}, (□A 🡒 ◇A) ∈ L) : (canonicalModel L).SerialMRel where
+  serial_mRel P := by
+    have h : ∀ C ∈ disjSet P.forbidden, C ∉ □⁻¹P.theory := by
+      rintro C ⟨K, hne, hsub, rfl⟩ hmem;
+      exact P.avoid (◇(⋁K)) ⟨⋁K, ⟨K, hne, hsub, rfl⟩, rfl⟩
+        (P.theory.mdp (P.theory.subset (L := L) hD) hmem);
+    obtain ⟨P₁, h₁, -, havoid⟩ :=
+      CanonicalPair.exists_avoiding (L := L) (T := □⁻¹P.theory) orDirected_disjSet h;
+    exact ⟨P₁, CanonicalPair.mRel_of_avoid_disjSet h₁ havoid⟩;
+
+end CK
+
+theorem LogicCKD_TFAE {A : BDFormula} : List.TFAE [
+  A ∈ LogicCKD,
+  A ∈ LogicCKPDia,
+  ∀ {κ : Type 0}, ∀ F : CK.Frame κ, [F.SerialMRel] → F ⊧ A,
+] := by
+  tfae_have 1 → 2 := LogicCKD.eq_CKPDia ▸ id
+  tfae_have 2 → 3 := fun h _ F _ V V_per V_fal =>
+    CK.Model.valid_of_mem_LogicCKD (LogicCKD.eq_CKPDia ▸ h)
+  tfae_have 3 → 1 := by
+    contrapose!;
+    intro h;
+    obtain ⟨P, h₁⟩ := CK.exists_not_forces_of_not_mem h;
+    refine ⟨_, (CK.canonicalModel LogicCKD).toFrame, ?_⟩;
+    and_intros;
+    . exact CK.serialMRel_canonicalModel (by grind);
+    . by_contra! hF;
+      exact h₁ $ CK.Model.valid_of_toFrame_valid hF P;
+  tfae_finish
+
+end
