NCML/CK/Logic/CKTBox.lean
@@ -1,0 +1,56 @@
+module
+
+public import NCML.CK.Frame.ReturningMRel
+public import NCML.CK.Canonical
+public import NCML.CK.Soundness
+
+@[expose] public section
+
+open ProvableBDHilbert
+
+namespace CK
+
+variable {κ : Type*} {M : Model κ}
+variable {A : BDFormula}
+
+namespace Model
+
+open CK.Frame
+
+lemma valid_of_mem_LogicCKTBox [M.TBox] (hA : A ∈ LogicCKTBox) : M ⊧ A :=
+  valid_of_mem_logic
+    (by rintro B ⟨C, rfl⟩; exact valid_of_toFrame_valid frameValidate_TBox_of_frame_TBox) hA
+
+end Model
+
+variable {L : BDLogic} [L.CK]
+
+lemma returningMRel_canonicalModel (hTBox : ∀ {A}, (□A 🡒 A) ∈ L) : (canonicalModel L).ReturningMRel where
+  returning_mRel P := ⟨
+    P.erase,
+    CanonicalPair.iRel_erase,
+    fun _ hA => P.theory.mdp (P.theory.subset (L := L) hTBox) hA,
+    by simp
+  ⟩
+
+end CK
+
+theorem LogicCKTBox_TFAE {A : BDFormula} : List.TFAE [
+  A ∈ LogicCKTBox,
+  ∀ {κ : Type 0}, ∀ F : CK.Frame κ, [F.TBox] → F ⊧ A,
+  ∀ {κ : Type 0}, ∀ F : CK.Frame κ, [F.ReturningMRel] → F ⊧ A,
+] := by
+  tfae_have 1 → 2 := fun h _ F _ V V_per V_fal => CK.Model.valid_of_mem_LogicCKTBox h
+  tfae_have 2 → 3 := fun h _ F _ => h F
+  tfae_have 3 → 1 := by
+    contrapose!;
+    intro h;
+    obtain ⟨P, h₁⟩ := CK.exists_not_forces_of_not_mem h;
+    refine ⟨_, (CK.canonicalModel LogicCKTBox).toFrame, ?_⟩;
+    and_intros;
+    . exact CK.returningMRel_canonicalModel (by grind);
+    . by_contra! hF;
+      exact h₁ $ CK.Model.valid_of_toFrame_valid hF P;
+  tfae_finish
+
+end
