NCML/CK/Logic/CKTDia.lean
@@ -1,0 +1,73 @@
+module
+
+public import NCML.CK.Frame.StrictlyAscendingMRel
+public import NCML.CK.Canonical
+public import NCML.CK.Soundness
+
+@[expose] public section
+
+open ProvableBDHilbert
+open scoped BDFormulaSet BDFormulaList
+
+namespace CK
+
+variable {κ : Type*} {M : Model κ}
+variable {A : BDFormula}
+
+namespace Model
+
+open CK.Frame
+
+lemma valid_of_mem_LogicCKTDia [M.TDia] (hA : A ∈ LogicCKTDia) : M ⊧ A :=
+  valid_of_mem_logic
+    (by rintro B ⟨C, rfl⟩; exact valid_of_toFrame_valid frameValidate_TDia_of_frame_TDia) hA
+
+end Model
+
+variable {L : BDLogic} [L.CK]
+
+private lemma avoid_disjSet_mdpClosure (hTDia : ∀ {A}, (A 🡒 ◇A) ∈ L) (P : CanonicalPair L) :
+  ∀ C ∈ disjSet P.forbidden, C ∉ BDTheory.mdpClosure (P.theory ∪ □⁻¹P.theory) := by
+  rintro C ⟨K, hne, hsub, rfl⟩ hmem;
+  obtain ⟨D, hD, E, hE, hDE⟩ := BDTheory.mdpClosure_union_finite_char hmem;
+  have h₁ : □(D 🡒 ⋁K) ∈ P.theory :=
+    P.theory.mdp (BDTheory.provable_mem (box_mono (mdp imp_swap hDE))) hE;
+  have h₂ : (◇D 🡒 ◇(⋁K)) ∈ P.theory := P.theory.mdp (BDTheory.provable_mem kDia) h₁;
+  have h₃ : ◇D ∈ P.theory := P.theory.mdp (P.theory.subset (L := L) hTDia) hD;
+  exact P.avoid (◇(⋁K)) ⟨⋁K, ⟨K, hne, hsub, rfl⟩, rfl⟩ (P.theory.mdp h₂ h₃);
+
+lemma strictlyAscendingMRel_canonicalModel (hTDia : ∀ {A}, (A 🡒 ◇A) ∈ L) :
+  (canonicalModel L).StrictlyAscendingMRel where
+  strictly_ascending_mRel P := by
+    have : BDTheory.Of L (P.theory ∪ □⁻¹P.theory) :=
+      ⟨(P.theory.subset (L := L)).trans Set.subset_union_left⟩;
+    obtain ⟨P₁, h₁, -, havoid⟩ :=
+      CanonicalPair.exists_avoiding (L := L) (T := BDTheory.mdpClosure (P.theory ∪ □⁻¹P.theory))
+      orDirected_disjSet (avoid_disjSet_mdpClosure hTDia P);
+    have h₂ : P.theory ∪ □⁻¹P.theory ⊆ P₁.theory := BDTheory.subset_mdpClosure.trans h₁;
+    use P₁;
+    constructor;
+    . exact CanonicalPair.mRel_of_avoid_disjSet (Set.subset_union_right.trans h₂) havoid;
+    . exact Set.subset_union_left.trans h₂;
+
+end CK
+
+theorem LogicCKTDia_TFAE {A : BDFormula} : List.TFAE [
+  A ∈ LogicCKTDia,
+  ∀ {κ : Type 0}, ∀ F : CK.Frame κ, [F.TDia] → F ⊧ A,
+  ∀ {κ : Type 0}, ∀ F : CK.Frame κ, [F.StrictlyAscendingMRel] → F ⊧ A,
+] := by
+  tfae_have 1 → 2 := fun h _ F _ V V_per V_fal => CK.Model.valid_of_mem_LogicCKTDia h
+  tfae_have 2 → 3 := fun h _ F _ => h F
+  tfae_have 3 → 1 := by
+    contrapose!;
+    intro h;
+    obtain ⟨P, h₁⟩ := CK.exists_not_forces_of_not_mem h;
+    refine ⟨_, (CK.canonicalModel LogicCKTDia).toFrame, ?_⟩;
+    and_intros;
+    . exact CK.strictlyAscendingMRel_canonicalModel (by grind);
+    . by_contra! hF;
+      exact h₁ $ CK.Model.valid_of_toFrame_valid hF P;
+  tfae_finish
+
+end
